src/tls/Record.fst
@@ -76,7 +76,7 @@ effect EXT (a:Type) = ST a
   (requires (fun _ -> True))
   (ensures (fun h0 _ h1 -> modifies Set.empty h0 h1))
 
-val read: Transport.networkStream -> EXT (result (contentType * protocolVersion * b:bytes { length b <= max_TLSCiphertext_fragment_length}))
+val read: Transport.t -> EXT (result (contentType * protocolVersion * b:bytes { length b <= max_TLSCiphertext_fragment_length}))
 
 // in the spirit of TLS 1.3, we ignore the outer protocol version (see appendix C):
 // our server never treats the ClientHello's record pv as its minimum supported pv;
